Coq/Wavefronts.v
@@ -12,6 +12,7 @@ Unset Printing Implicit Defensive.
    lemmas about them. *)
 (*******************************************************************************)
 
+
 Section Wavefronts.
 
 (* Definition of a wavefront *)
@@ -21,17 +22,9 @@ Definition wavefront (l : log) :=
 (* Default log entry *)
 Variable e0 : LogEntry.
 
-Definition prefix (l : log) := {l1 | exists n, l1 = take n l}.
-
-Program Definition take_prefix (n' : nat) l : prefix l.
-Proof. by apply: (exist _ (take n' l)); exists n'. Defined.
-
 (* An alternative definition of a log decomposition procedure *)
 Fixpoint prefixes_rec (l : log) n := 
-  if n is n'.+1 
-  then (take_prefix n' l, nth e0 l n', n') :: prefixes_rec l n' 
-  else [::].
-
+  if n is n'.+1 then (take n' l, nth e0 l n', n') :: prefixes_rec l n' else [::].
 Definition prefixes l := prefixes_rec l (size l).
 
 (* Some properties of our selector function "prefixes". *)
@@ -44,42 +37,93 @@ rewrite -[n.+1]addn1 -[(size s).+1]addn1 ltn_add2r=>/IHs=>H.
 by rewrite addn1 -{4}H.
 Qed.
 
-Lemma prefixes_in' l e j n :
+(* Adequacy of prefixes *)
+
+Lemma in_prefixes_full l e pr i: (pr, e, i) \in prefixes l ->
+  [/\ i < size l, nth e0 l i = e & pr = take i l].
+Proof.
+rewrite /prefixes.
+elim: (size l)=>//=n Hi.
+case/orP; last first.
+- by case/Hi=>H1 H2; split=>//; apply: (ltn_trans H1); apply:ltnSn.
+by case/eqP=>Z1 Z2 Z3; subst pr e i.
+Qed.
+
+Lemma in_prefixes l e pr i: (pr, e, i) \in prefixes l -> e \in l.
+Proof.
+case/in_prefixes_full=>H1 H2.
+have X: exists2 j, j < size l & nth e0 l j = e by exists i=>//.
+by move/nthP: X.
+Qed.
+
+Lemma prefixes_in' l e j n : 
   e \in l -> j < n -> nth e0 l j = e ->
-  (take_prefix j l, e, j) \In prefixes_rec l n.
+  (take j l, e, j) \in prefixes_rec l n.
 Proof.
 elim: n=>//=n Hi H1 H2 H3; case B: (j == n).
-move/eqP: B=>B; subst j. 
-- by apply/In_cons; left; rewrite H3.
+- by move/eqP: B=>B; subst j; rewrite inE H3 eqxx.
 have X: j < n by rewrite ltnS leq_eqVlt B/= in H2.
-by apply/In_cons; right; move:(Hi H1 X H3).
+by rewrite inE; move:(Hi H1 X H3)=>->; rewrite orbC.
+Qed.
+
+Lemma prefixes_in l e: e \in l -> 
+  exists i, (take i l, e, i) \in prefixes l.
+Proof.
+by move=>D; case/(nthP e0): (D)=>j H1 H2; exists j; apply: prefixes_in'.
+Qed.
+
+Lemma prefixes_num' l j n  : 
+  j < n -> n <= size l -> exists e, (take j l, e, j) \in prefixes_rec l n.
+Proof.
+elim: n=>//=n Hi H1 H2; case B: (j == n); last first.
+- have X: j < n by rewrite ltnS leq_eqVlt B/= in H1.
+  have Y: n <= size l by apply:ltnW. 
+  by case: (Hi X Y)=>e G; exists e; rewrite inE G orbC.
+move/eqP: B=>B; subst j=>{H1 Hi}.
+exists (nth e0 l n).
+by rewrite inE eqxx.
+Qed.
+
+Lemma prefixes_num l n  : 
+  n < size l -> exists e, (take n l, e, n) \in prefixes l.
+Proof.
+by move/(@prefixes_num' l n (size l))=>H; apply:H; apply:leqnn.
+Qed.
+
+Lemma prefV l pr e n:
+  (pr, e, n) \in prefixes l -> 
+  [/\ pr = take n l, 
+      e = (nth e0 l n) & 
+      l = pr ++ e :: drop n.+1 l].
+Proof.
+move=>H; case: (in_prefixes_full H)=>G1 G2 G3.
+by rewrite G3 -G2; split=>//; move: (take_nth_drop G1)=>->.
 Qed.
 
 Lemma prefix_rev l1 l2 l et e :
   e \in l2 -> l = l1 ++ et :: l2  ->
-  exists i, (take_prefix i l, e, i) \In prefixes l /\ 
-            et \in take i l.
+  exists i, (take i l, e, i) \in prefixes l /\ et \in take i l.
 Proof.
 case/splitP=>{l2}l2 l3.
 rewrite -cat_cons -cats1 cat_cons -catA cat1s -cat_cons catA.
 set i := size (l1 ++ et :: l2); move=>E; exists i.
-have X1 : e \in l by rewrite E mem_cat inE eqxx orbC.
+have X1 : e \in l by rewrite E mem_cat inE eqxx orbC.  
 have X2: i < size l
-  by rewrite/i E!size_cat -addnA ltn_add2l -{1}[size (_::l2)]addn0 ltn_add2l.
+  by rewrite/i E!size_cat -addnA ltn_add2l -{1}[size (_::l2)]addn0 ltn_add2l. 
 have Y: forall a, a - a = 0 by elim.
-have X3: nth e0 l i = e by rewrite E nth_cat /i ltnn Y/=.
+have X3: nth e0 l i = e by rewrite E nth_cat /i ltnn Y/=. 
 move: (prefixes_in' X1 X2 X3)=>H; split=>//.
 by rewrite E take_size_cat /i// mem_cat inE eqxx orbC.
 Qed.
 
 Lemma prefix_wavefront l1 l2 l et e :
   e \in l2 -> l = l1 ++ et :: l2  -> kind et == T ->
-  exists i pre, (pre, e, i) \In prefixes l /\
-                (source et, fld et) \in (wavefront (proj1_sig pre)).
+  exists i pre, (pre, e, i) \in prefixes l /\ 
+                (source et, fld et) \in (wavefront pre).
 Proof.
 move=>H1 H2 T; case:(prefix_rev H1 H2)=>i[H3 H4].
-exists i, (take_prefix i l); split=>//.
-by apply/mapP; exists et=>//; rewrite mem_filter T.
+exists i, (take i l); split=>//.
+by apply/mapP; exists et=>//; rewrite mem_filter T. 
 Qed.
 
 Lemma wavefront_trace l o : o \in wavefront l ->
@@ -90,90 +134,5 @@ case/mapP=>e; rewrite mem_filter=>/andP[H1].
 by case/in_split=>l1[l2][E]->/=; exists e, l1, l2.
 Qed.
 
-(* Adequacy of prefixes *)
-
-(* Lemma in_prefixes_full l e pr i: (pr, e, i) \in prefixes l -> *)
-(*   [/\ i < size l, nth e0 l i = e & pr = take i l]. *)
-(* Proof. *)
-(* rewrite /prefixes. *)
-(* elim: (size l)=>//=n Hi. *)
-(* case/orP; last first. *)
-(* - by case/Hi=>H1 H2; split=>//; apply: (ltn_trans H1); apply:ltnSn. *)
-(* by case/eqP=>Z1 Z2 Z3; subst pr e i. *)
-(* Qed. *)
-
-(* Lemma in_prefixes l e pr i: (pr, e, i) \in prefixes l -> e \in l. *)
-(* Proof. *)
-(* case/in_prefixes_full=>H1 H2. *)
-(* have X: exists2 j, j < size l & nth e0 l j = e by exists i=>//. *)
-(* by move/nthP: X. *)
-(* Qed. *)
-
-
-(* Lemma prefixes_in l e: e \in l ->  *)
-(*   exists i, (take i l, e, i) \in prefixes l. *)
-(* Proof. *)
-(* by move=>D; case/(nthP e0): (D)=>j H1 H2; exists j; apply: prefixes_in'. *)
-(* Qed. *)
-
-(* Lemma prefixes_num' l j n  :  *)
-(*   j < n -> n <= size l -> exists e, (take j l, e, j) \in prefixes_rec l n. *)
-(* Proof. *)
-(* elim: n=>//=n Hi H1 H2; case B: (j == n); last first. *)
-(* - have X: j < n by rewrite ltnS leq_eqVlt B/= in H1. *)
-(*   have Y: n <= size l by apply:ltnW.  *)
-(*   by case: (Hi X Y)=>e G; exists e; rewrite inE G orbC. *)
-(* move/eqP: B=>B; subst j=>{H1 Hi}. *)
-(* exists (nth e0 l n). *)
-(* by rewrite inE eqxx. *)
-(* Qed. *)
-
-(* Lemma prefixes_num l n  :  *)
-(*   n < size l -> exists e, (take n l, e, n) \in prefixes l. *)
-(* Proof. *)
-(* by move/(@prefixes_num' l n (size l))=>H; apply:H; apply:leqnn. *)
-(* Qed. *)
-
-(* Lemma prefV l pr e n: *)
-(*   (pr, e, n) \in prefixes l ->  *)
-(*   [/\ pr = take n l,  *)
-(*       e = (nth e0 l n) &  *)
-(*       l = pr ++ e :: drop n.+1 l]. *)
-(* Proof. *)
-(* move=>H; case: (in_prefixes_full H)=>G1 G2 G3. *)
-(* by rewrite G3 -G2; split=>//; move: (take_nth_drop G1)=>->. *)
-(* Qed. *)
-
 End Wavefronts.
 
-
-(*******************************************************************************)
-(*       Helper functions to work with sequences of refinement types           *)
-(*******************************************************************************)
-
-
-Lemma mapP' {A : Type} {B : eqType} (f : A -> B) s y : 
-     reflect (exists x, x \In s /\ y = f x) (y \in map f s).
-Proof.
-elim: s => [|x s IHs].
-- by rewrite /= in_nil; constructor; case=>x[/In_nil]. 
-rewrite in_cons eq_sym; case Hxy: (f x == y).
-- by constructor; exists x; move/eqP:Hxy=>->; split=>//; apply/In_cons; left.
-apply: (iffP IHs).
-- by case=>z[H1 H2]; exists z; split=>//; apply/In_cons; right.
-move=>[x'[Hx' Dy]]; move: Dy Hxy=>->. 
-by case/In_cons: Hx'=>[->|H]; [by rewrite eqxx|by exists x']. 
-Qed.
-
-Lemma mem_filter' {A : Type} (a : A -> bool) x s : 
-   a x /\ (x \In s) -> (x \In filter a s).
-Proof.
-case=>H; elim: s; first by case=>_/In_nil.
-move=>/= y s IHs.
-rewrite (fun_if (fun s' : seq A => x \In s'))=>/In_cons.
-case=>H1; last first; case: ifP.
-- by move=>_; apply/In_cons; right; apply: IHs.
-- by move=>_; apply: IHs.
-- by subst y=>_; apply/In_cons; left.
-by subst y; rewrite H.
-Qed.
